fix type of wp_pred_pair

deps/poulet4/lib/P4automata/WP.v
@@ -177,7 +177,7 @@ Section WP.
   Definition wp_pred_pair
              (phi: conf_rel a)
              (preds: nat * (state_template a * state_template a))
-    : list (conf_rel a) :=
+    : conf_rel a :=
     let '(size, (prev_l, prev_r)) := preds in
     let phi_rel := phi.(cr_rel) in
     let cur_l := phi.(cr_st).(cs_st1) in
@@ -186,11 +186,11 @@ Section WP.
     let leap_r := leap_kind prev_r cur_r in
     let b := (BEVar H (BVarTop phi.(cr_ctx) size)) in
     let phi_rel := weaken_store_rel size phi_rel in
-    [{| cr_st := {| cs_st1 := prev_l;
-                    cs_st2 := prev_r |};
-        cr_rel := wp_lpred Left b prev_l cur_l leap_l
-                           (wp_lpred Right b prev_r cur_r leap_r phi_rel) |}].
-
+    {| cr_st := {| cs_st1 := prev_l;
+                   cs_st2 := prev_r |};
+       cr_rel := wp_lpred Left b prev_l cur_l leap_l
+                          (wp_lpred Right b prev_r cur_r leap_r phi_rel) |}.
+  
   Definition reaches (cur prev: state_template a * state_template a) : list (nat * (state_template a * state_template a)) :=
     let '(n, successors) := Reachability.reachable_pair_step' prev in
     if List.In_dec (Reachability.state_pair_eq_dec (a := a))
@@ -203,37 +203,7 @@ Section WP.
     let cur_st_left  := phi.(cr_st).(cs_st1) in
     let cur_st_right := phi.(cr_st).(cs_st2) in
     let pred_pairs := List.flat_map (reaches (cur_st_left, cur_st_right)) reachable_states in
-    List.flat_map (wp_pred_pair phi) pred_pairs.
-
-
-  (*
-S is a relation on pairs
-x, y in wp(S)
-<->
-there exists a string of bits bs
-such that x--[bs]-->x'
-      and y--[bs]-->y'
-with x', y' in S.
-*)
-(*
-s1 {
-  extract(h, 1)
-  if (h)
-    goto s2
-  else
-    goto s3
-}
-s2 {
-  goto accept
-}
-s3 {
-  goto accept
-}
-
-
-what is wp(<s2, s2> |- false) ?
-<s1, s1> |- h = 0
-*)
+    List.map (wp_pred_pair phi) pred_pairs.
 
 End WP.
 
